WIP Z reification fails

src/Arithmetic/SolinasReduction.v
@@ -104,7 +104,7 @@ End Z.
 
 Module stream.
   Local Open Scope nat_scope.
-  Definition stream T := nat -> T.
+  Notation stream := (fun T => nat -> T).
   Definition hd {T} (xs : stream T) : T := xs O.
   Definition tl {T} (xs : stream T) : stream T := fun i => xs (S i).
   Definition skipn {T} n (xs : stream T) : stream T := fun i => xs (n+i).
@@ -144,22 +144,22 @@ Module Saturated. Section __.
   Import Positional List ListNotations.
   Import stream Coq.Init.Datatypes Coq.Lists.List List.
 
-  Implicit Types (weight bound : stream positive).
-  Local Open Scope positive_scope.
+  Implicit Types (weight bound : stream Z).
+  Local Open Scope Z_scope.
 
-  Definition weight bound := stream.map (fold_right Pos.mul xH) (stream.prefixes bound).
+  Definition weight bound := stream.map (fold_right Z.mul 1) (stream.prefixes bound).
 
-  Lemma weight_0 bound : weight bound O = 1%positive. Proof. trivial. Qed.
+  Lemma weight_0 bound : weight bound O = 1%Z. Proof. trivial. Qed.
 
   Lemma weight_1 bound : weight bound 1%nat = bound O. Proof. cbn. lia. Qed.
 
   Lemma tl_weight bound i : stream.tl (weight bound) i = stream.hd bound * weight (stream.tl bound) i.
   Proof. cbv [weight]. rewrite tl_map. cbv [stream.map]. rewrite tl_prefixes; trivial. Qed.
 
-  Lemma tl_weight' bound i : stream.tl (weight bound) i = (weight bound i * bound i)%positive.
+  Lemma tl_weight' bound i : stream.tl (weight bound) i = (weight bound i * bound i)%Z.
   Proof.
     cbv [stream.tl weight stream.prefixes stream.map].
-    rewrite stream.firstn_S', fold_right_app; cbn [fold_right]; rewrite Pos.prod_init; lia.
+    rewrite stream.firstn_S', fold_right_app; cbn [fold_right]; rewrite Z.prod_init; lia.
   Qed.
 
   (*
@@ -209,8 +209,10 @@ Module Saturated. Section __.
     { rewrite weight_0. ring_simplify; trivial. }
     setoid_rewrite IHxs; clear IHxs.
     ring_simplify; f_equal.
-    rewrite !(Z.mul_comm _ (eval _ _)), <-Pos2Z.inj_mul, <-tl_weight; trivial.
+    (*
+    rewrite !(Z.mul_comm _ (eval _ _)), <-Z2Z.inj_mul, <-tl_weight; trivial.
   Qed.
+     *)Admitted.
 
   Definition encode bound (n : nat) (x : Z) : list Z :=
     nat_rect _ (fun _ _ => []) (fun _ rec x bound =>
@@ -237,12 +239,14 @@ Module Saturated. Section __.
     revert x; revert dependent bound; induction n; intros;
       rewrite ?encode_O, ?encode_S, ?eval_nil, ?eval_cons.
     { rewrite ?weight_0, Z.mod_1_r; trivial. }
-    setoid_rewrite IHn. setoid_rewrite tl_weight. rewrite ?Pos2Z.inj_mul.
+    (*
+    setoid_rewrite IHn. setoid_rewrite tl_weight. rewrite ?Z2Z.inj_mul.
     set (Z.pos (stream.hd bound)) as B in *.
     symmetry; rewrite (Z.div_mod x B), Z.add_comm at 1 by lia.
     rewrite <-Z.add_mod_idemp_r, Zmult_mod_distr_l by lia.
     apply Z.mod_small; Z.div_mod_to_equations; nia.
   Qed.
+     *)Admitted.
 
   Lemma encode_add_l bound n m x :
     encode bound (n+m) x = encode bound n x ++ encode (stream.skipn n bound) m (x / weight bound n).
@@ -251,12 +255,14 @@ Module Saturated. Section __.
       rewrite ?encode_O, ?encode_S.
     { rewrite weight_0, Z.div_1_r. reflexivity. }
     setoid_rewrite IHn; cbn [app]; f_equal.
-    rewrite Z.div_div, <-Pos2Z.inj_mul, <-tl_weight by lia.
+    (*
+    rewrite Z.div_div, <-Z2Z.inj_mul, <-tl_weight by lia.
     { (* setoid_rewrite stream.skipn_tl *)
       eapply f_equal2; [reflexivity|].
       eapply Proper_encode; [|reflexivity..].
       intro i; eapply stream.skipn_tl. }
   Qed.
+     *)Admitted.
 
   Lemma firstn_encode bound i n x (H : Nat.lt i n) :
     firstn i (encode bound n x) = encode bound i x.
@@ -280,12 +286,14 @@ Module Saturated. Section __.
     eval (stream.skipn i bound) (skipn i (encode bound n x)) = x mod weight bound n / weight bound i.
   Proof.
     rewrite skipn_encode, eval_encode; trivial.
+    (*
     rewrite Z.mod_pull_div by lia.
     f_equal.
     f_equal.
-    rewrite <-Pos2Z.inj_mul.
+    rewrite <-Z2Z.inj_mul.
     f_equal.
   Admitted.
+     *)Admitted.
 
   Definition add bound (c0 : Z) (xs ys : list Z) : list Z * Z  :=
     list_rect _ (fun _ _ c => ([], c)) (fun x _  rec bound ys c =>
@@ -318,10 +326,12 @@ Module Saturated. Section __.
     rewrite IHxs by ( rewrite length_tl; lia); clear IHxs.
     repeat (apply (f_equal2 pair) || apply (f_equal2 cons)).
     { push_Zmod; pull_Zmod. f_equal. rewrite Z.mul_0_l, Z.add_0_r. lia. }
+    (*
     { f_equal. Z.div_mod_to_equations; nia. }
     { setoid_rewrite tl_weight.
       rewrite <-2Z.div_add, Z.div_div; f_equal; lia. }
   Qed.
+     *)Admitted.
 
   (* See lemma saturated_pseudomersenne_reduction_converges *)
 
@@ -346,7 +356,7 @@ Module Saturated. Section __.
     set (weight bound k) as W.
 
     epose proof (saturated_pseudomersenne_reduction_converges W s c (@eval bound a) b).
-    progress change (Z.pos (weight bound (length a))) with s.
+    progress change ((weight bound (length a))) with s.
     subst W.
     subst s.
     rewrite eval_skipn_encode by trivial.
@@ -362,6 +372,7 @@ Module Saturated. Section __.
     rewrite <-Z.div_mod by lia.
     push_Zmod; rewrite Hc; pull_Zmod.
     trivial.
+    all: fail.
   Admitted.
 
   Definition addmod bound c a b :=
@@ -380,29 +391,31 @@ Module Saturated. Section __.
     rewrite <-eval_reduce'; rewrite ?eval_encode, ?length_encode, ?weight_1;
       try solve [trivial | cbn; lia | apply Z.mod_pos_bound; lia ].
     { rewrite (Z.add_comm (_ mod _) (_ * (_ / _))), <-Z.div_mod; lia. }
+    (*
     assert (Z.abs ((eval bound a + eval bound b) / Z.pos (weight bound (length a))) <= 1) by (Z.div_mod_to_equations; nia); nia.
   Qed.
+     *)Admitted.
 
   Local Notation "!" := ltac:(vm_decide) (only parsing).
   Goal forall a0 a1 a2 a3 b : Z, False. intros.
   Proof.
-    pose proof (eval_reduce' (fun _ => 2^64)%positive 1 38 [a0;a1;a2;a3] b (2^256-38) ! ! ! !).
+    pose proof (eval_reduce' (fun _ => 2^64)%Z 1 38 [a0;a1;a2;a3] b (2^256-38) ! ! ! !).
     cbn [length] in *.
-    change (Z.pos (weight (fun _ : nat => (2 ^ 64)%positive) 4%nat)) with (2^256) in *.
-    change (Z.pos (weight (fun _ : nat => (2 ^ 64)%positive) 1%nat)) with (2^64) in *.
-    change (weight (fun _ : nat => (2 ^ 64)%positive) 1%nat)%positive with (2^64)%positive in *.
-    set (eval (fun _ : nat => (2 ^ 64)%positive)) as eval in *.
-    set (reduce' (fun _ : nat => (2 ^ 64)%positive) _ _ _) as reduce' in *.
+    change ((weight (fun _ : nat => (2 ^ 64)%Z) 4%nat)) with (2^256) in *.
+    change ((weight (fun _ : nat => (2 ^ 64)%Z) 1%nat)) with (2^64) in *.
+    change (weight (fun _ : nat => (2 ^ 64)%Z) 1%nat)%Z with (2^64)%Z in *.
+    set (eval (fun _ : nat => (2 ^ 64)%Z)) as eval in *.
+    set (reduce' (fun _ : nat => (2 ^ 64)%Z) _ _ _) as reduce' in *.
   Abort.
 
   Goal forall a0 a1 a2 a3 b0 b1 b2 b3 : Z, False. intros.
   Proof.
-    pose proof (eval_addmod (fun _ => 2^64)%positive 38 [a0;a1;a2;a3] [b0;b1;b2;b3] (2^256-38) ! ! ! !).
+    pose proof (eval_addmod (fun _ => 2^64)%Z 38 [a0;a1;a2;a3] [b0;b1;b2;b3] (2^256-38) ! ! ! !).
     cbn [length] in *.
-    change (Z.pos (weight (fun _ : nat => (2 ^ 64)%positive) 4%nat)) with (2^256) in *.
-    change (Z.pos (weight (fun _ : nat => (2 ^ 64)%positive) 1%nat)) with (2^64) in *.
-    change (weight (fun _ : nat => (2 ^ 64)%positive) 1%nat)%positive with (2^64)%positive in *.
-    set (eval (fun _ : nat => (2 ^ 64)%positive)) as eval in *.
+    change ((weight (fun _ : nat => (2 ^ 64)%Z) 4%nat)) with (2^256) in *.
+    change ((weight (fun _ : nat => (2 ^ 64)%Z) 1%nat)) with (2^64) in *.
+    change (weight (fun _ : nat => (2 ^ 64)%Z) 1%nat)%Z with (2^64)%Z in *.
+    set (eval (fun _ : nat => (2 ^ 64)%Z)) as eval in *.
     set (addmod _ _) as addmod in *.
   Abort.
 End __.
